Splinter/SequenceSets.i.dfy
@@ -1,0 +1,7 @@
+// TODO move into lib someday
+module SequenceSetsMod {
+  predicate SequenceSubset<T>(a:seq<T>, b:seq<T>)
+  {
+    forall i | 0<=i<|a| :: a[i] in b
+  }
+}
